change to tree-shaped isla

frontend/coq_pp.ml
@@ -301,43 +301,50 @@ let pp_event ff e =
 
 (** [pp_trace_def name] is a pretty-printer for the Coq definition of a trace,
 with given definition name [name]. *)
-let pp_trace : trace Format.pp = fun ff (Trace events) ->
+let pp_events : event list Format.pp = fun ff events ->
   let pp fmt = Format.fprintf ff fmt in
-  pp "@[<v 2>[";
-  let print_event =
-    let first = ref true in
-    let print_event e =
-      (if !first then first := false else pp ";");
-      pp "@;%a" pp_event e
-    in
-    print_event
+  let print_event e =
+    pp "@;%a :t:" pp_event e
   in
-  List.iter print_event events;
-  pp ("@]" ^^ (if events = [] then "" else "@;") ^^ "]")
+  List.iter print_event events
 
-let pp_traces_def : string -> traces Format.pp = fun id ff (Traces trcs) ->
+let rec pp_forking_trace : trace Format.pp = fun ff (ForkingTrace(trcs, cont)) ->
   let pp fmt = Format.fprintf ff fmt in
-  pp "@[<v 2>Definition %s : list trc := [" id;
-  let print_trace =
-    let first = ref true in
-    let print_trace t =
-      (if !first then first := false else pp ";");
-      pp "@;%a" pp_trace t
-    in
-    print_trace
-  in
-  List.iter print_trace (List.sort Stdlib.compare trcs);
-  pp "@]@;]."
+  pp "%a" pp_events trcs;
+  pp "%a" pp_maybe_fork cont
+
+and pp_maybe_fork : maybe_fork Format.pp = fun ff mf ->
+  let pp fmt = Format.fprintf ff fmt in
+  match mf with
+  | Ast.Fork(n, trcs) ->
+     pp "@;@[<v 2>tfork [";
+     let print_trace =
+       let first = ref true in
+       let print_trace e =
+         (if !first then first := false else pp ";");
+         pp "%a" pp_forking_trace e
+       in
+       print_trace
+     in
+     List.iter print_trace trcs;
+     pp "@]@;]"
+  | Ast.NoFork        -> pp "@;tnil"
+
+let pp_traces_def : string -> trace Format.pp = fun id ff trc ->
+  let pp fmt = Format.fprintf ff fmt in
+  pp "@[<v 2>Definition %s : isla_trace :=" id;
+  pp "%a" pp_forking_trace trc;
+  pp "@]@;."
 
 
 (** [pp_trace_file name] is the entry point of the pretty-printer. [name] is the name
 of the generated Definition. *)
-let pp_traces_file : string -> traces Format.pp = fun id ff trs ->
+let pp_traces_file : string -> trace Format.pp = fun id ff trs ->
   let pp fmt = Format.fprintf ff fmt in
-  pp "@[<v 0>From isla Require Import isla_lang.@;@;";
+  pp "@[<v 0>From isla Require Import opsem.@;@;";
   pp "%a@]" (pp_traces_def id) trs
 
-let write_traces_to_file : string -> traces -> string -> unit = fun id trs fname ->
+let write_traces_to_file : string -> trace -> string -> unit = fun id trs fname ->
   let buffer = Buffer.create 4096 in
   Format.fprintf (Format.formatter_of_buffer buffer) "%a@." (pp_traces_file id) trs;
   (* Check if we should write the file (inexistent / contents different). *)
@@ -347,7 +354,7 @@ let write_traces_to_file : string -> traces -> string -> unit = fun id trs fname
   in
   if must_write then Buffer.to_file fname buffer
 
-let write_traces : string -> traces -> string option -> unit = fun id tr fname ->
+let write_traces : string -> trace -> string option -> unit = fun id tr fname ->
   match fname with
   | Some(fname) -> write_traces_to_file id tr fname
   | None        -> Format.printf "%a@." (pp_traces_file id) tr
