frontend/isla_lang_if.ml
@@ -1,71 +1,26 @@
 module Ast = Isla_lang.AST
 
-type event = unit Ast.event
-type trace = unit Ast.trc
-type traces = unit Ast.trcs
+type event = Ast.lrng Ast.event
+type trace = Ast.lrng Ast.forking_trc
+type maybe_fork = Ast.lrng Ast.maybe_fork
 
 (** [filter_events pred trs] returns a copy of [trs] in which only events that
     satisfy the predicate [pred] have been kept. *)
-let filter_events : (event -> bool) -> traces -> traces = fun pred trs ->
+let filter_events : (event -> bool) -> trace -> trace = fun pred trs ->
   let open Ast in
-  let filter_trace (Trace(tr)) = Trace(List.filter pred tr) in
-  let filter_traces (Traces(trs)) = Traces(List.map filter_trace trs) in
-  filter_traces trs
-
-let erase_traces : 'a Ast.trcs -> traces =
-  let open Ast in
-  let rec erase_a_exp e =
-    match e with
-    | AExp_Val(v,_)       -> AExp_Val(v, ())
-    | AExp_Unop(o,e,_)    -> AExp_Unop(o, erase_a_exp e, ())
-    | AExp_Binop(o,x,y,_) -> AExp_Binop(o, erase_a_exp x,erase_a_exp y, ())
-    | AExp_Manyop(o,es,_) -> AExp_Manyop(o, List.map erase_a_exp es, ())
-    | AExp_Ite(x,y,z,_)   -> AExp_Ite(erase_a_exp x, erase_a_exp y,
-                              erase_a_exp z, ())
+  let rec filter_trace (ForkingTrace(trs, mf)) =
+    ForkingTrace(List.filter pred trs, filter_maybe_fork mf)
+  and filter_maybe_fork mf =
+    match mf with
+    | Fork(n, trcs) -> Fork(n, List.map filter_trace trcs)
+    | NoFork    -> NoFork
   in
-  let rec erase_exp e =
-    match e with
-    | Val(v,_)       -> Val(v, ())
-    | Unop(o,e,_)    -> Unop(o, erase_exp e, ())
-    | Binop(o,x,y,_) -> Binop(o, erase_exp x,erase_exp y, ())
-    | Manyop(o,es,_) -> Manyop(o, List.map erase_exp es, ())
-    | Ite(x,y,z,_)   -> Ite(erase_exp x, erase_exp y, erase_exp z, ())
-  in
-  let erase_smt s =
-    match s with
-    | DeclareConst(i,ty) -> DeclareConst(i, ty)
-    | DefineConst(i,e)   -> DefineConst(i, erase_exp e)
-    | Assert(e)          -> Assert(erase_exp e)
-    | DefineEnum(i)      -> DefineEnum(i)
-  in
-  let erase_event e =
-    match e with
-    | Smt(s,_)                 -> Smt(erase_smt s, ())
-    | Branch(i,s,_)            -> Branch(i, s, ())
-    | ReadReg(s,l,v,_)         -> ReadReg(s, l, v, ())
-    | WriteReg(s,l,v,_)        -> WriteReg(s, l, v, ())
-    | ReadMem(a,b,c,i,vo,_)    -> ReadMem(a, b, c, i, vo, ())
-    | WriteMem(a,b,c,d,i,vo,_) -> WriteMem(a, b, c, d, i, vo, ())
-    | BranchAddress(v,_)       -> BranchAddress(v, ())
-    | Barrier(v,_)             -> Barrier(v, ())
-    | CacheOp(v,w,_)           -> CacheOp(v, w, ())
-    | MarkReg(s,t,_)           -> MarkReg(s, t, ())
-    | Cycle(_)                 -> Cycle(())
-    | Instr(v,_)               -> Instr(v, ())
-    | Sleeping(i,_)            -> Sleeping(i, ())
-    | WakeRequest(_)           -> WakeRequest(())
-    | SleepRequest(_)          -> SleepRequest(())
-    | AssumeReg(s,l,v,_)       -> AssumeReg(s, l, v, ())
-    | Assume(e,_)              -> Assume(erase_a_exp e, ())
-  in
-  let erase_trace (Trace es) = Trace (List.map erase_event es) in
-  let erase_traces (Traces trs) = Traces (List.map erase_trace trs) in
-  erase_traces
+  filter_trace trs
 
 module Parser = struct
   exception Parse_error of string
 
-  let parse_file : string -> traces = fun fname ->
+  let parse_file : string -> trace = fun fname ->
     let module L = Isla_lang.Lexer in
     let module P = Isla_lang.Parser in
     let fail fmt =
@@ -84,8 +39,9 @@ module Parser = struct
     let ic = try open_in fname with Sys_error(msg) -> fail "%s" msg in
     let lexbuf = Lexing.from_channel ic in
     try
-      let ast = P.trcs_start L.token lexbuf in
-      close_in ic; erase_traces ast
+      let ast = P.forking_trc_start L.token lexbuf in
+      close_in ic;
+      ast
     with e ->
     close_in ic;
     match e with
@@ -99,53 +55,3 @@ module Parser = struct
     | e            ->
         fail "Unexpected exception: %s." (Printexc.to_string e)
 end
-
-let compare : traces -> traces -> int =
-  let open Ast in
-  let rec erase_a_exp e =
-    match e with
-    | AExp_Val(v,_)       -> AExp_Val(v, ())
-    | AExp_Unop(o,e,_)    -> AExp_Unop(o, erase_a_exp e, ())
-    | AExp_Binop(o,x,y,_) -> AExp_Binop(o, erase_a_exp x,erase_a_exp y, ())
-    | AExp_Manyop(o,es,_) -> AExp_Manyop(o, List.map erase_a_exp es, ())
-    | AExp_Ite(x,y,z,_)   -> AExp_Ite(erase_a_exp x, erase_a_exp y,
-                              erase_a_exp z, ())
-  in
-  let rec erase_exp e =
-    match e with
-    | Val(v,_)       -> Val(v, ())
-    | Unop(o,e,_)    -> Unop(o, erase_exp e, ())
-    | Binop(o,x,y,_) -> Binop(o, erase_exp x,erase_exp y, ())
-    | Manyop(o,es,_) -> Manyop(o, List.map erase_exp es, ())
-    | Ite(x,y,z,_)   -> Ite(erase_exp x, erase_exp y, erase_exp z, ())
-  in
-  let erase_smt s =
-    match s with
-    | DeclareConst(i,ty) -> DeclareConst(i, ty)
-    | DefineConst(i,e)   -> DefineConst(i, erase_exp e)
-    | Assert(e)          -> Assert(erase_exp e)
-    | DefineEnum(i)      -> DefineEnum(i)
-  in
-  let erase_event e =
-    match e with
-    | Smt(s,_)                 -> Smt(erase_smt s, ())
-    | Branch(i,s,_)            -> Branch(i, s, ())
-    | ReadReg(s,l,v,_)         -> ReadReg(s, l, v, ())
-    | WriteReg(s,l,v,_)        -> WriteReg(s, l, v, ())
-    | ReadMem(a,b,c,i,vo,_)    -> ReadMem(a, b, c, i, vo, ())
-    | WriteMem(a,b,c,d,i,vo,_) -> WriteMem(a, b, c, d, i, vo, ())
-    | BranchAddress(v,_)       -> BranchAddress(v, ())
-    | Barrier(v,_)             -> Barrier(v, ())
-    | CacheOp(v,w,_)           -> CacheOp(v, w, ())
-    | MarkReg(s,t,_)           -> MarkReg(s, t, ())
-    | Cycle(_)                 -> Cycle(())
-    | Instr(v,_)               -> Instr(v, ())
-    | Sleeping(i,_)            -> Sleeping(i, ())
-    | WakeRequest(_)           -> WakeRequest(())
-    | SleepRequest(_)          -> SleepRequest(())
-    | AssumeReg(s,l,v,_)       -> AssumeReg(s, l, v, ())
-    | Assume(e,_)              -> Assume(erase_a_exp e, ())
-  in
-  let erase_trace (Trace es) = Trace (List.map erase_event es) in
-  let erase_traces (Traces trs) = Traces (List.map erase_trace trs) in
-  fun trs1 trs2 -> Stdlib.compare (erase_traces trs1) (erase_traces trs2)
