instructions/binary_search/a54.v
@@ -1,31 +1,30 @@
-From isla Require Import isla_lang.
+From isla Require Import opsem.
 
-Definition a54 : list trc := [
-  [
-    AssumeReg "HCR_EL2" [] (RegVal_Base (Val_Bits [BV{64%N} 0x80000000%Z])) Mk_annot;
-    AssumeReg "CFG_ID_AA64PFR0_EL1_EL3" [] (RegVal_Base (Val_Bits [BV{4%N} 0x1%Z])) Mk_annot;
-    AssumeReg "CFG_ID_AA64PFR0_EL1_EL2" [] (RegVal_Base (Val_Bits [BV{4%N} 0x1%Z])) Mk_annot;
-    AssumeReg "CFG_ID_AA64PFR0_EL1_EL1" [] (RegVal_Base (Val_Bits [BV{4%N} 0x1%Z])) Mk_annot;
-    AssumeReg "CFG_ID_AA64PFR0_EL1_EL0" [] (RegVal_Base (Val_Bits [BV{4%N} 0x1%Z])) Mk_annot;
-    AssumeReg "TCR_EL2" [] (RegVal_Base (Val_Bits [BV{64%N} 0x0%Z])) Mk_annot;
-    AssumeReg "PSTATE" [Field "EL"] (RegVal_Base (Val_Bits [BV{2%N} 0x2%Z])) Mk_annot;
-    AssumeReg "PSTATE" [Field "nRW"] (RegVal_Base (Val_Bits [BV{1%N} 0x0%Z])) Mk_annot;
-    AssumeReg "SCR_EL3" [] (RegVal_Base (Val_Bits [BV{32%N} 0x401%Z])) Mk_annot;
-    Smt (DeclareConst 47%Z (Ty_BitVec 64%N)) Mk_annot;
-    ReadReg "_PC" [] (RegVal_Base (Val_Symbolic 47%Z)) Mk_annot;
-    Smt (DefineConst 48%Z (Manyop (Bvmanyarith Bvadd) [Val (Val_Symbolic 47%Z) Mk_annot; Val (Val_Bits [BV{64%N} 0x8%Z]) Mk_annot] Mk_annot)) Mk_annot;
-    ReadReg "PSTATE" [Field "nRW"] (RegVal_Struct [("nRW", RegVal_Base (Val_Bits [BV{1%N} 0x0%Z]))]) Mk_annot;
-    ReadReg "CFG_ID_AA64PFR0_EL1_EL0" [] (RegVal_Base (Val_Bits [BV{4%N} 0x1%Z])) Mk_annot;
-    ReadReg "CFG_ID_AA64PFR0_EL1_EL1" [] (RegVal_Base (Val_Bits [BV{4%N} 0x1%Z])) Mk_annot;
-    ReadReg "CFG_ID_AA64PFR0_EL1_EL2" [] (RegVal_Base (Val_Bits [BV{4%N} 0x1%Z])) Mk_annot;
-    ReadReg "CFG_ID_AA64PFR0_EL1_EL3" [] (RegVal_Base (Val_Bits [BV{4%N} 0x1%Z])) Mk_annot;
-    Smt (DefineConst 49%Z (Val (Val_Symbolic 48%Z) Mk_annot)) Mk_annot;
-    BranchAddress (RegVal_Base (Val_Symbolic 49%Z)) Mk_annot;
-    Smt (DefineConst 50%Z (Val (Val_Symbolic 48%Z) Mk_annot)) Mk_annot;
-    ReadReg "PSTATE" [Field "EL"] (RegVal_Struct [("EL", RegVal_Base (Val_Bits [BV{2%N} 0x2%Z]))]) Mk_annot;
-    ReadReg "SCR_EL3" [] (RegVal_Base (Val_Bits [BV{32%N} 0x401%Z])) Mk_annot;
-    ReadReg "HCR_EL2" [] (RegVal_Base (Val_Bits [BV{64%N} 0x80000000%Z])) Mk_annot;
-    ReadReg "TCR_EL2" [] (RegVal_Base (Val_Bits [BV{64%N} 0x0%Z])) Mk_annot;
-    WriteReg "_PC" [] (RegVal_Base (Val_Symbolic 50%Z)) Mk_annot
-  ]
-].
+Definition a54 : isla_trace :=
+  AssumeReg "HCR_EL2" [] (RegVal_Base (Val_Bits [BV{64%N} 0x80000000%Z])) Mk_annot :t:
+  AssumeReg "CFG_ID_AA64PFR0_EL1_EL3" [] (RegVal_Base (Val_Bits [BV{4%N} 0x1%Z])) Mk_annot :t:
+  AssumeReg "CFG_ID_AA64PFR0_EL1_EL2" [] (RegVal_Base (Val_Bits [BV{4%N} 0x1%Z])) Mk_annot :t:
+  AssumeReg "CFG_ID_AA64PFR0_EL1_EL1" [] (RegVal_Base (Val_Bits [BV{4%N} 0x1%Z])) Mk_annot :t:
+  AssumeReg "CFG_ID_AA64PFR0_EL1_EL0" [] (RegVal_Base (Val_Bits [BV{4%N} 0x1%Z])) Mk_annot :t:
+  AssumeReg "TCR_EL2" [] (RegVal_Base (Val_Bits [BV{64%N} 0x0%Z])) Mk_annot :t:
+  AssumeReg "PSTATE" [Field "EL"] (RegVal_Base (Val_Bits [BV{2%N} 0x2%Z])) Mk_annot :t:
+  AssumeReg "PSTATE" [Field "nRW"] (RegVal_Base (Val_Bits [BV{1%N} 0x0%Z])) Mk_annot :t:
+  AssumeReg "SCR_EL3" [] (RegVal_Base (Val_Bits [BV{32%N} 0x401%Z])) Mk_annot :t:
+  Smt (DeclareConst 47%Z (Ty_BitVec 64%N)) Mk_annot :t:
+  ReadReg "_PC" [] (RegVal_Base (Val_Symbolic 47%Z)) Mk_annot :t:
+  Smt (DefineConst 48%Z (Manyop (Bvmanyarith Bvadd) [Val (Val_Symbolic 47%Z) Mk_annot; Val (Val_Bits [BV{64%N} 0x8%Z]) Mk_annot] Mk_annot)) Mk_annot :t:
+  ReadReg "PSTATE" [Field "nRW"] (RegVal_Struct [("nRW", RegVal_Base (Val_Bits [BV{1%N} 0x0%Z]))]) Mk_annot :t:
+  ReadReg "CFG_ID_AA64PFR0_EL1_EL0" [] (RegVal_Base (Val_Bits [BV{4%N} 0x1%Z])) Mk_annot :t:
+  ReadReg "CFG_ID_AA64PFR0_EL1_EL1" [] (RegVal_Base (Val_Bits [BV{4%N} 0x1%Z])) Mk_annot :t:
+  ReadReg "CFG_ID_AA64PFR0_EL1_EL2" [] (RegVal_Base (Val_Bits [BV{4%N} 0x1%Z])) Mk_annot :t:
+  ReadReg "CFG_ID_AA64PFR0_EL1_EL3" [] (RegVal_Base (Val_Bits [BV{4%N} 0x1%Z])) Mk_annot :t:
+  Smt (DefineConst 49%Z (Val (Val_Symbolic 48%Z) Mk_annot)) Mk_annot :t:
+  BranchAddress (RegVal_Base (Val_Symbolic 49%Z)) Mk_annot :t:
+  Smt (DefineConst 50%Z (Val (Val_Symbolic 48%Z) Mk_annot)) Mk_annot :t:
+  ReadReg "PSTATE" [Field "EL"] (RegVal_Struct [("EL", RegVal_Base (Val_Bits [BV{2%N} 0x2%Z]))]) Mk_annot :t:
+  ReadReg "SCR_EL3" [] (RegVal_Base (Val_Bits [BV{32%N} 0x401%Z])) Mk_annot :t:
+  ReadReg "HCR_EL2" [] (RegVal_Base (Val_Bits [BV{64%N} 0x80000000%Z])) Mk_annot :t:
+  ReadReg "TCR_EL2" [] (RegVal_Base (Val_Bits [BV{64%N} 0x0%Z])) Mk_annot :t:
+  WriteReg "_PC" [] (RegVal_Base (Val_Symbolic 50%Z)) Mk_annot :t:
+  tnil
+.
