instructions/binary_search/ac.v
@@ -1,76 +1,75 @@
-From isla Require Import isla_lang.
+From isla Require Import opsem.
 
-Definition ac : list trc := [
-  [
-    AssumeReg "HCR_EL2" [] (RegVal_Base (Val_Bits [BV{64%N} 0x80000000%Z])) Mk_annot;
-    AssumeReg "CFG_ID_AA64PFR0_EL1_EL3" [] (RegVal_Base (Val_Bits [BV{4%N} 0x1%Z])) Mk_annot;
-    AssumeReg "CFG_ID_AA64PFR0_EL1_EL2" [] (RegVal_Base (Val_Bits [BV{4%N} 0x1%Z])) Mk_annot;
-    AssumeReg "CFG_ID_AA64PFR0_EL1_EL1" [] (RegVal_Base (Val_Bits [BV{4%N} 0x1%Z])) Mk_annot;
-    AssumeReg "CFG_ID_AA64PFR0_EL1_EL0" [] (RegVal_Base (Val_Bits [BV{4%N} 0x1%Z])) Mk_annot;
-    AssumeReg "TCR_EL2" [] (RegVal_Base (Val_Bits [BV{64%N} 0x0%Z])) Mk_annot;
-    AssumeReg "EDSCR" [] (RegVal_Base (Val_Bits [BV{32%N} 0x0%Z])) Mk_annot;
-    AssumeReg "OSDLR_EL1" [] (RegVal_Base (Val_Bits [BV{32%N} 0x0%Z])) Mk_annot;
-    AssumeReg "OSLSR_EL1" [] (RegVal_Base (Val_Bits [BV{32%N} 0x0%Z])) Mk_annot;
-    Smt (DeclareConst 6%Z (Ty_BitVec 1%N)) Mk_annot;
-    AssumeReg "PSTATE" [Field "EL"] (RegVal_Base (Val_Bits [BV{2%N} 0x2%Z])) Mk_annot;
-    AssumeReg "PSTATE" [Field "SP"] (RegVal_Base (Val_Bits [BV{1%N} 0x1%Z])) Mk_annot;
-    AssumeReg "PSTATE" [Field "nRW"] (RegVal_Base (Val_Bits [BV{1%N} 0x0%Z])) Mk_annot;
-    AssumeReg "SCR_EL3" [] (RegVal_Base (Val_Bits [BV{32%N} 0x401%Z])) Mk_annot;
-    AssumeReg "SCTLR_EL2" [] (RegVal_Base (Val_Bits [BV{64%N} 0x4000002%Z])) Mk_annot;
-    Smt (DeclareConst 29%Z (Ty_BitVec 64%N)) Mk_annot;
-    Assume (AExp_Binop (Eq) (AExp_Manyop (Bvmanyarith Bvand) [AExp_Val (AVal_Var "SP_EL2" []) Mk_annot; AExp_Val (AVal_Bits [BV{64%N} 0xfff0000000000007%Z]) Mk_annot] Mk_annot) (AExp_Val (AVal_Bits [BV{64%N} 0x0%Z]) Mk_annot) Mk_annot) Mk_annot;
-    Smt (Assert (Binop (Eq) (Manyop (Bvmanyarith Bvand) [Val (Val_Symbolic 29%Z) Mk_annot; Val (Val_Bits [BV{64%N} 0xfff0000000000007%Z]) Mk_annot] Mk_annot) (Val (Val_Bits [BV{64%N} 0x0%Z]) Mk_annot) Mk_annot)) Mk_annot;
-    Assume (AExp_Binop (Eq) (AExp_Manyop (Bvmanyarith Bvand) [AExp_Manyop (Bvmanyarith Bvadd) [AExp_Val (AVal_Var "SP_EL2" []) Mk_annot; AExp_Val (AVal_Bits [BV{64%N} 0x38%Z]) Mk_annot] Mk_annot; AExp_Val (AVal_Bits [BV{64%N} 0xfff0000000000007%Z]) Mk_annot] Mk_annot) (AExp_Val (AVal_Bits [BV{64%N} 0x0%Z]) Mk_annot) Mk_annot) Mk_annot;
-    Smt (Assert (Binop (Eq) (Manyop (Bvmanyarith Bvand) [Manyop (Bvmanyarith Bvadd) [Val (Val_Symbolic 29%Z) Mk_annot; Val (Val_Bits [BV{64%N} 0x38%Z]) Mk_annot] Mk_annot; Val (Val_Bits [BV{64%N} 0xfff0000000000007%Z]) Mk_annot] Mk_annot) (Val (Val_Bits [BV{64%N} 0x0%Z]) Mk_annot) Mk_annot)) Mk_annot;
-    ReadReg "PSTATE" [Field "SP"] (RegVal_Struct [("SP", RegVal_Base (Val_Bits [BV{1%N} 0x1%Z]))]) Mk_annot;
-    ReadReg "PSTATE" [Field "EL"] (RegVal_Struct [("EL", RegVal_Base (Val_Bits [BV{2%N} 0x2%Z]))]) Mk_annot;
-    ReadReg "SP_EL2" [] (RegVal_Base (Val_Symbolic 29%Z)) Mk_annot;
-    ReadReg "SCTLR_EL2" [] (RegVal_Base (Val_Bits [BV{64%N} 0x4000002%Z])) Mk_annot;
-    Smt (DefineConst 73%Z (Manyop (Bvmanyarith Bvadd) [Val (Val_Symbolic 29%Z) Mk_annot; Val (Val_Bits [BV{64%N} 0x30%Z]) Mk_annot] Mk_annot)) Mk_annot;
-    Smt (DeclareConst 74%Z (Ty_BitVec 64%N)) Mk_annot;
-    ReadReg "R20" [] (RegVal_Base (Val_Symbolic 74%Z)) Mk_annot;
-    Smt (DefineConst 75%Z (Val (Val_Symbolic 74%Z) Mk_annot)) Mk_annot;
-    Smt (DeclareConst 76%Z (Ty_BitVec 64%N)) Mk_annot;
-    ReadReg "R19" [] (RegVal_Base (Val_Symbolic 76%Z)) Mk_annot;
-    Smt (DefineConst 77%Z (Val (Val_Symbolic 76%Z) Mk_annot)) Mk_annot;
-    Smt (DefineConst 78%Z (Manyop (Bvmanyarith Bvadd) [Val (Val_Symbolic 73%Z) Mk_annot; Val (Val_Bits [BV{64%N} 0x0%Z]) Mk_annot] Mk_annot)) Mk_annot;
-    ReadReg "PSTATE" [Field "nRW"] (RegVal_Struct [("nRW", RegVal_Base (Val_Bits [BV{1%N} 0x0%Z]))]) Mk_annot;
-    ReadReg "CFG_ID_AA64PFR0_EL1_EL0" [] (RegVal_Base (Val_Bits [BV{4%N} 0x1%Z])) Mk_annot;
-    ReadReg "CFG_ID_AA64PFR0_EL1_EL1" [] (RegVal_Base (Val_Bits [BV{4%N} 0x1%Z])) Mk_annot;
-    ReadReg "CFG_ID_AA64PFR0_EL1_EL2" [] (RegVal_Base (Val_Bits [BV{4%N} 0x1%Z])) Mk_annot;
-    ReadReg "CFG_ID_AA64PFR0_EL1_EL3" [] (RegVal_Base (Val_Bits [BV{4%N} 0x1%Z])) Mk_annot;
-    Smt (DefineConst 83%Z (Binop (Eq) (Val (Val_Symbolic 78%Z) Mk_annot) (Manyop (Bvmanyarith Bvand) [Val (Val_Symbolic 78%Z) Mk_annot; Val (Val_Bits [BV{64%N} 0xfffffffffffffff8%Z]) Mk_annot] Mk_annot) Mk_annot)) Mk_annot;
-    Smt (Assert (Unop (Not) (Unop (Not) (Val (Val_Symbolic 83%Z) Mk_annot) Mk_annot) Mk_annot)) Mk_annot;
-    Smt (Assert (Unop (Not) (Unop (Not) (Val (Val_Symbolic 83%Z) Mk_annot) Mk_annot) Mk_annot)) Mk_annot;
-    Smt (Assert (Binop (Eq) (Val (Val_Symbolic 78%Z) Mk_annot) (Manyop (Bvmanyarith Bvand) [Val (Val_Symbolic 78%Z) Mk_annot; Val (Val_Bits [BV{64%N} 0xfffffffffffffff8%Z]) Mk_annot] Mk_annot) Mk_annot)) Mk_annot;
-    ReadReg "SCR_EL3" [] (RegVal_Base (Val_Bits [BV{32%N} 0x401%Z])) Mk_annot;
-    ReadReg "HCR_EL2" [] (RegVal_Base (Val_Bits [BV{64%N} 0x80000000%Z])) Mk_annot;
-    ReadReg "TCR_EL2" [] (RegVal_Base (Val_Bits [BV{64%N} 0x0%Z])) Mk_annot;
-    Smt (Assert (Unop (Not) (Unop (Not) (Binop (Eq) (Unop (Extract 63%N 52%N) (Val (Val_Symbolic 78%Z) Mk_annot) Mk_annot) (Val (Val_Bits [BV{12%N} 0x0%Z]) Mk_annot) Mk_annot) Mk_annot) Mk_annot)) Mk_annot;
-    Smt (Assert (Unop (Not) (Unop (Not) (Val (Val_Symbolic 83%Z) Mk_annot) Mk_annot) Mk_annot)) Mk_annot;
-    ReadReg "PSTATE" [Field "D"] (RegVal_Struct [("D", RegVal_Base (Val_Symbolic 6%Z))]) Mk_annot;
-    ReadReg "OSLSR_EL1" [] (RegVal_Base (Val_Bits [BV{32%N} 0x0%Z])) Mk_annot;
-    ReadReg "OSDLR_EL1" [] (RegVal_Base (Val_Bits [BV{32%N} 0x0%Z])) Mk_annot;
-    ReadReg "EDSCR" [] (RegVal_Base (Val_Bits [BV{32%N} 0x0%Z])) Mk_annot;
-    Smt (DeclareConst 1261%Z (Ty_BitVec 64%N)) Mk_annot;
-    ReadReg "MPIDR_EL1" [] (RegVal_Base (Val_Symbolic 1261%Z)) Mk_annot;
-    Smt (DeclareConst 1330%Z (Ty_BitVec 56%N)) Mk_annot;
-    Smt (DefineConst 1343%Z (Unop (ZeroExtend 8%N) (Manyop Concat [Val (Val_Bits [BV{4%N} 0x0%Z]) Mk_annot; Unop (Extract 51%N 0%N) (Val (Val_Symbolic 78%Z) Mk_annot) Mk_annot] Mk_annot) Mk_annot)) Mk_annot;
-    Smt (DeclareConst 1344%Z Ty_Bool) Mk_annot;
-    WriteMem (RegVal_Base (Val_Symbolic 1344%Z)) (RegVal_Base (Val_Enum ((Mk_enum_id 6%nat), Mk_enum_ctor 0%nat))) (RegVal_Base (Val_Symbolic 1343%Z)) (RegVal_Base (Val_Symbolic 75%Z)) 8%N None Mk_annot;
-    Smt (DefineConst 1345%Z (Manyop (Bvmanyarith Bvadd) [Val (Val_Symbolic 73%Z) Mk_annot; Val (Val_Bits [BV{64%N} 0x8%Z]) Mk_annot] Mk_annot)) Mk_annot;
-    Smt (DefineConst 1350%Z (Binop (Eq) (Val (Val_Symbolic 1345%Z) Mk_annot) (Manyop (Bvmanyarith Bvand) [Val (Val_Symbolic 1345%Z) Mk_annot; Val (Val_Bits [BV{64%N} 0xfffffffffffffff8%Z]) Mk_annot] Mk_annot) Mk_annot)) Mk_annot;
-    Smt (Assert (Unop (Not) (Unop (Not) (Val (Val_Symbolic 1350%Z) Mk_annot) Mk_annot) Mk_annot)) Mk_annot;
-    Smt (Assert (Unop (Not) (Unop (Not) (Val (Val_Symbolic 1350%Z) Mk_annot) Mk_annot) Mk_annot)) Mk_annot;
-    Smt (Assert (Binop (Eq) (Val (Val_Symbolic 1345%Z) Mk_annot) (Manyop (Bvmanyarith Bvand) [Val (Val_Symbolic 1345%Z) Mk_annot; Val (Val_Bits [BV{64%N} 0xfffffffffffffff8%Z]) Mk_annot] Mk_annot) Mk_annot)) Mk_annot;
-    Smt (Assert (Unop (Not) (Unop (Not) (Binop (Eq) (Unop (Extract 63%N 52%N) (Val (Val_Symbolic 1345%Z) Mk_annot) Mk_annot) (Val (Val_Bits [BV{12%N} 0x0%Z]) Mk_annot) Mk_annot) Mk_annot) Mk_annot)) Mk_annot;
-    Smt (Assert (Unop (Not) (Unop (Not) (Val (Val_Symbolic 1350%Z) Mk_annot) Mk_annot) Mk_annot)) Mk_annot;
-    Smt (DefineConst 2575%Z (Unop (ZeroExtend 8%N) (Manyop Concat [Val (Val_Bits [BV{4%N} 0x0%Z]) Mk_annot; Unop (Extract 51%N 0%N) (Val (Val_Symbolic 1345%Z) Mk_annot) Mk_annot] Mk_annot) Mk_annot)) Mk_annot;
-    Smt (DeclareConst 2576%Z Ty_Bool) Mk_annot;
-    WriteMem (RegVal_Base (Val_Symbolic 2576%Z)) (RegVal_Base (Val_Enum ((Mk_enum_id 6%nat), Mk_enum_ctor 0%nat))) (RegVal_Base (Val_Symbolic 2575%Z)) (RegVal_Base (Val_Symbolic 77%Z)) 8%N None Mk_annot;
-    Smt (DeclareConst 2577%Z (Ty_BitVec 64%N)) Mk_annot;
-    ReadReg "_PC" [] (RegVal_Base (Val_Symbolic 2577%Z)) Mk_annot;
-    Smt (DefineConst 2578%Z (Manyop (Bvmanyarith Bvadd) [Val (Val_Symbolic 2577%Z) Mk_annot; Val (Val_Bits [BV{64%N} 0x4%Z]) Mk_annot] Mk_annot)) Mk_annot;
-    WriteReg "_PC" [] (RegVal_Base (Val_Symbolic 2578%Z)) Mk_annot
-  ]
-].
+Definition ac : isla_trace :=
+  AssumeReg "HCR_EL2" [] (RegVal_Base (Val_Bits [BV{64%N} 0x80000000%Z])) Mk_annot :t:
+  AssumeReg "CFG_ID_AA64PFR0_EL1_EL3" [] (RegVal_Base (Val_Bits [BV{4%N} 0x1%Z])) Mk_annot :t:
+  AssumeReg "CFG_ID_AA64PFR0_EL1_EL2" [] (RegVal_Base (Val_Bits [BV{4%N} 0x1%Z])) Mk_annot :t:
+  AssumeReg "CFG_ID_AA64PFR0_EL1_EL1" [] (RegVal_Base (Val_Bits [BV{4%N} 0x1%Z])) Mk_annot :t:
+  AssumeReg "CFG_ID_AA64PFR0_EL1_EL0" [] (RegVal_Base (Val_Bits [BV{4%N} 0x1%Z])) Mk_annot :t:
+  AssumeReg "TCR_EL2" [] (RegVal_Base (Val_Bits [BV{64%N} 0x0%Z])) Mk_annot :t:
+  AssumeReg "EDSCR" [] (RegVal_Base (Val_Bits [BV{32%N} 0x0%Z])) Mk_annot :t:
+  AssumeReg "OSDLR_EL1" [] (RegVal_Base (Val_Bits [BV{32%N} 0x0%Z])) Mk_annot :t:
+  AssumeReg "OSLSR_EL1" [] (RegVal_Base (Val_Bits [BV{32%N} 0x0%Z])) Mk_annot :t:
+  Smt (DeclareConst 6%Z (Ty_BitVec 1%N)) Mk_annot :t:
+  AssumeReg "PSTATE" [Field "EL"] (RegVal_Base (Val_Bits [BV{2%N} 0x2%Z])) Mk_annot :t:
+  AssumeReg "PSTATE" [Field "SP"] (RegVal_Base (Val_Bits [BV{1%N} 0x1%Z])) Mk_annot :t:
+  AssumeReg "PSTATE" [Field "nRW"] (RegVal_Base (Val_Bits [BV{1%N} 0x0%Z])) Mk_annot :t:
+  AssumeReg "SCR_EL3" [] (RegVal_Base (Val_Bits [BV{32%N} 0x401%Z])) Mk_annot :t:
+  AssumeReg "SCTLR_EL2" [] (RegVal_Base (Val_Bits [BV{64%N} 0x4000002%Z])) Mk_annot :t:
+  Smt (DeclareConst 29%Z (Ty_BitVec 64%N)) Mk_annot :t:
+  Assume (AExp_Binop (Eq) (AExp_Manyop (Bvmanyarith Bvand) [AExp_Val (AVal_Var "SP_EL2" []) Mk_annot; AExp_Val (AVal_Bits [BV{64%N} 0xfff0000000000007%Z]) Mk_annot] Mk_annot) (AExp_Val (AVal_Bits [BV{64%N} 0x0%Z]) Mk_annot) Mk_annot) Mk_annot :t:
+  Smt (Assert (Binop (Eq) (Manyop (Bvmanyarith Bvand) [Val (Val_Symbolic 29%Z) Mk_annot; Val (Val_Bits [BV{64%N} 0xfff0000000000007%Z]) Mk_annot] Mk_annot) (Val (Val_Bits [BV{64%N} 0x0%Z]) Mk_annot) Mk_annot)) Mk_annot :t:
+  Assume (AExp_Binop (Eq) (AExp_Manyop (Bvmanyarith Bvand) [AExp_Manyop (Bvmanyarith Bvadd) [AExp_Val (AVal_Var "SP_EL2" []) Mk_annot; AExp_Val (AVal_Bits [BV{64%N} 0x38%Z]) Mk_annot] Mk_annot; AExp_Val (AVal_Bits [BV{64%N} 0xfff0000000000007%Z]) Mk_annot] Mk_annot) (AExp_Val (AVal_Bits [BV{64%N} 0x0%Z]) Mk_annot) Mk_annot) Mk_annot :t:
+  Smt (Assert (Binop (Eq) (Manyop (Bvmanyarith Bvand) [Manyop (Bvmanyarith Bvadd) [Val (Val_Symbolic 29%Z) Mk_annot; Val (Val_Bits [BV{64%N} 0x38%Z]) Mk_annot] Mk_annot; Val (Val_Bits [BV{64%N} 0xfff0000000000007%Z]) Mk_annot] Mk_annot) (Val (Val_Bits [BV{64%N} 0x0%Z]) Mk_annot) Mk_annot)) Mk_annot :t:
+  ReadReg "PSTATE" [Field "SP"] (RegVal_Struct [("SP", RegVal_Base (Val_Bits [BV{1%N} 0x1%Z]))]) Mk_annot :t:
+  ReadReg "PSTATE" [Field "EL"] (RegVal_Struct [("EL", RegVal_Base (Val_Bits [BV{2%N} 0x2%Z]))]) Mk_annot :t:
+  ReadReg "SP_EL2" [] (RegVal_Base (Val_Symbolic 29%Z)) Mk_annot :t:
+  ReadReg "SCTLR_EL2" [] (RegVal_Base (Val_Bits [BV{64%N} 0x4000002%Z])) Mk_annot :t:
+  Smt (DefineConst 73%Z (Manyop (Bvmanyarith Bvadd) [Val (Val_Symbolic 29%Z) Mk_annot; Val (Val_Bits [BV{64%N} 0x30%Z]) Mk_annot] Mk_annot)) Mk_annot :t:
+  Smt (DeclareConst 74%Z (Ty_BitVec 64%N)) Mk_annot :t:
+  ReadReg "R20" [] (RegVal_Base (Val_Symbolic 74%Z)) Mk_annot :t:
+  Smt (DefineConst 75%Z (Val (Val_Symbolic 74%Z) Mk_annot)) Mk_annot :t:
+  Smt (DeclareConst 76%Z (Ty_BitVec 64%N)) Mk_annot :t:
+  ReadReg "R19" [] (RegVal_Base (Val_Symbolic 76%Z)) Mk_annot :t:
+  Smt (DefineConst 77%Z (Val (Val_Symbolic 76%Z) Mk_annot)) Mk_annot :t:
+  Smt (DefineConst 78%Z (Manyop (Bvmanyarith Bvadd) [Val (Val_Symbolic 73%Z) Mk_annot; Val (Val_Bits [BV{64%N} 0x0%Z]) Mk_annot] Mk_annot)) Mk_annot :t:
+  ReadReg "PSTATE" [Field "nRW"] (RegVal_Struct [("nRW", RegVal_Base (Val_Bits [BV{1%N} 0x0%Z]))]) Mk_annot :t:
+  ReadReg "CFG_ID_AA64PFR0_EL1_EL0" [] (RegVal_Base (Val_Bits [BV{4%N} 0x1%Z])) Mk_annot :t:
+  ReadReg "CFG_ID_AA64PFR0_EL1_EL1" [] (RegVal_Base (Val_Bits [BV{4%N} 0x1%Z])) Mk_annot :t:
+  ReadReg "CFG_ID_AA64PFR0_EL1_EL2" [] (RegVal_Base (Val_Bits [BV{4%N} 0x1%Z])) Mk_annot :t:
+  ReadReg "CFG_ID_AA64PFR0_EL1_EL3" [] (RegVal_Base (Val_Bits [BV{4%N} 0x1%Z])) Mk_annot :t:
+  Smt (DefineConst 83%Z (Binop (Eq) (Val (Val_Symbolic 78%Z) Mk_annot) (Manyop (Bvmanyarith Bvand) [Val (Val_Symbolic 78%Z) Mk_annot; Val (Val_Bits [BV{64%N} 0xfffffffffffffff8%Z]) Mk_annot] Mk_annot) Mk_annot)) Mk_annot :t:
+  Smt (Assert (Unop (Not) (Unop (Not) (Val (Val_Symbolic 83%Z) Mk_annot) Mk_annot) Mk_annot)) Mk_annot :t:
+  Smt (Assert (Unop (Not) (Unop (Not) (Val (Val_Symbolic 83%Z) Mk_annot) Mk_annot) Mk_annot)) Mk_annot :t:
+  Smt (Assert (Binop (Eq) (Val (Val_Symbolic 78%Z) Mk_annot) (Manyop (Bvmanyarith Bvand) [Val (Val_Symbolic 78%Z) Mk_annot; Val (Val_Bits [BV{64%N} 0xfffffffffffffff8%Z]) Mk_annot] Mk_annot) Mk_annot)) Mk_annot :t:
+  ReadReg "SCR_EL3" [] (RegVal_Base (Val_Bits [BV{32%N} 0x401%Z])) Mk_annot :t:
+  ReadReg "HCR_EL2" [] (RegVal_Base (Val_Bits [BV{64%N} 0x80000000%Z])) Mk_annot :t:
+  ReadReg "TCR_EL2" [] (RegVal_Base (Val_Bits [BV{64%N} 0x0%Z])) Mk_annot :t:
+  Smt (Assert (Unop (Not) (Unop (Not) (Binop (Eq) (Unop (Extract 63%N 52%N) (Val (Val_Symbolic 78%Z) Mk_annot) Mk_annot) (Val (Val_Bits [BV{12%N} 0x0%Z]) Mk_annot) Mk_annot) Mk_annot) Mk_annot)) Mk_annot :t:
+  Smt (Assert (Unop (Not) (Unop (Not) (Val (Val_Symbolic 83%Z) Mk_annot) Mk_annot) Mk_annot)) Mk_annot :t:
+  ReadReg "PSTATE" [Field "D"] (RegVal_Struct [("D", RegVal_Base (Val_Symbolic 6%Z))]) Mk_annot :t:
+  ReadReg "OSLSR_EL1" [] (RegVal_Base (Val_Bits [BV{32%N} 0x0%Z])) Mk_annot :t:
+  ReadReg "OSDLR_EL1" [] (RegVal_Base (Val_Bits [BV{32%N} 0x0%Z])) Mk_annot :t:
+  ReadReg "EDSCR" [] (RegVal_Base (Val_Bits [BV{32%N} 0x0%Z])) Mk_annot :t:
+  Smt (DeclareConst 1261%Z (Ty_BitVec 64%N)) Mk_annot :t:
+  ReadReg "MPIDR_EL1" [] (RegVal_Base (Val_Symbolic 1261%Z)) Mk_annot :t:
+  Smt (DeclareConst 1330%Z (Ty_BitVec 56%N)) Mk_annot :t:
+  Smt (DefineConst 1343%Z (Unop (ZeroExtend 8%N) (Manyop Concat [Val (Val_Bits [BV{4%N} 0x0%Z]) Mk_annot; Unop (Extract 51%N 0%N) (Val (Val_Symbolic 78%Z) Mk_annot) Mk_annot] Mk_annot) Mk_annot)) Mk_annot :t:
+  Smt (DeclareConst 1344%Z Ty_Bool) Mk_annot :t:
+  WriteMem (RegVal_Base (Val_Symbolic 1344%Z)) (RegVal_Base (Val_Enum ((Mk_enum_id 6%nat), Mk_enum_ctor 0%nat))) (RegVal_Base (Val_Symbolic 1343%Z)) (RegVal_Base (Val_Symbolic 75%Z)) 8%N None Mk_annot :t:
+  Smt (DefineConst 1345%Z (Manyop (Bvmanyarith Bvadd) [Val (Val_Symbolic 73%Z) Mk_annot; Val (Val_Bits [BV{64%N} 0x8%Z]) Mk_annot] Mk_annot)) Mk_annot :t:
+  Smt (DefineConst 1350%Z (Binop (Eq) (Val (Val_Symbolic 1345%Z) Mk_annot) (Manyop (Bvmanyarith Bvand) [Val (Val_Symbolic 1345%Z) Mk_annot; Val (Val_Bits [BV{64%N} 0xfffffffffffffff8%Z]) Mk_annot] Mk_annot) Mk_annot)) Mk_annot :t:
+  Smt (Assert (Unop (Not) (Unop (Not) (Val (Val_Symbolic 1350%Z) Mk_annot) Mk_annot) Mk_annot)) Mk_annot :t:
+  Smt (Assert (Unop (Not) (Unop (Not) (Val (Val_Symbolic 1350%Z) Mk_annot) Mk_annot) Mk_annot)) Mk_annot :t:
+  Smt (Assert (Binop (Eq) (Val (Val_Symbolic 1345%Z) Mk_annot) (Manyop (Bvmanyarith Bvand) [Val (Val_Symbolic 1345%Z) Mk_annot; Val (Val_Bits [BV{64%N} 0xfffffffffffffff8%Z]) Mk_annot] Mk_annot) Mk_annot)) Mk_annot :t:
+  Smt (Assert (Unop (Not) (Unop (Not) (Binop (Eq) (Unop (Extract 63%N 52%N) (Val (Val_Symbolic 1345%Z) Mk_annot) Mk_annot) (Val (Val_Bits [BV{12%N} 0x0%Z]) Mk_annot) Mk_annot) Mk_annot) Mk_annot)) Mk_annot :t:
+  Smt (Assert (Unop (Not) (Unop (Not) (Val (Val_Symbolic 1350%Z) Mk_annot) Mk_annot) Mk_annot)) Mk_annot :t:
+  Smt (DefineConst 2575%Z (Unop (ZeroExtend 8%N) (Manyop Concat [Val (Val_Bits [BV{4%N} 0x0%Z]) Mk_annot; Unop (Extract 51%N 0%N) (Val (Val_Symbolic 1345%Z) Mk_annot) Mk_annot] Mk_annot) Mk_annot)) Mk_annot :t:
+  Smt (DeclareConst 2576%Z Ty_Bool) Mk_annot :t:
+  WriteMem (RegVal_Base (Val_Symbolic 2576%Z)) (RegVal_Base (Val_Enum ((Mk_enum_id 6%nat), Mk_enum_ctor 0%nat))) (RegVal_Base (Val_Symbolic 2575%Z)) (RegVal_Base (Val_Symbolic 77%Z)) 8%N None Mk_annot :t:
+  Smt (DeclareConst 2577%Z (Ty_BitVec 64%N)) Mk_annot :t:
+  ReadReg "_PC" [] (RegVal_Base (Val_Symbolic 2577%Z)) Mk_annot :t:
+  Smt (DefineConst 2578%Z (Manyop (Bvmanyarith Bvadd) [Val (Val_Symbolic 2577%Z) Mk_annot; Val (Val_Bits [BV{64%N} 0x4%Z]) Mk_annot] Mk_annot)) Mk_annot :t:
+  WriteReg "_PC" [] (RegVal_Base (Val_Symbolic 2578%Z)) Mk_annot :t:
+  tnil
+.
