instructions/hello/a0.v
@@ -1,12 +1,11 @@
-From isla Require Import isla_lang.
+From isla Require Import opsem.
 
-Definition a0 : list trc := [
-  [
-    Smt (DeclareConst 37%Z (Ty_BitVec 64%N)) Mk_annot;
-    ReadReg "_PC" [] (RegVal_Base (Val_Symbolic 37%Z)) Mk_annot;
-    Smt (DefineConst 40%Z (Manyop (Bvmanyarith Bvadd) [Manyop (Bvmanyarith Bvor) [Manyop (Bvmanyarith Bvand) [Val (Val_Symbolic 37%Z) Mk_annot; Val (Val_Bits [BV{64%N} 0xfffffffffffff000%Z]) Mk_annot] Mk_annot; Val (Val_Bits [BV{64%N} 0x0%Z]) Mk_annot] Mk_annot; Val (Val_Bits [BV{64%N} 0x0%Z]) Mk_annot] Mk_annot)) Mk_annot;
-    WriteReg "R1" [] (RegVal_Base (Val_Symbolic 40%Z)) Mk_annot;
-    Smt (DefineConst 41%Z (Manyop (Bvmanyarith Bvadd) [Val (Val_Symbolic 37%Z) Mk_annot; Val (Val_Bits [BV{64%N} 0x4%Z]) Mk_annot] Mk_annot)) Mk_annot;
-    WriteReg "_PC" [] (RegVal_Base (Val_Symbolic 41%Z)) Mk_annot
-  ]
-].
+Definition a0 : isla_trace :=
+  Smt (DeclareConst 37%Z (Ty_BitVec 64%N)) Mk_annot :t:
+  ReadReg "_PC" [] (RegVal_Base (Val_Symbolic 37%Z)) Mk_annot :t:
+  Smt (DefineConst 40%Z (Manyop (Bvmanyarith Bvadd) [Manyop (Bvmanyarith Bvor) [Manyop (Bvmanyarith Bvand) [Val (Val_Symbolic 37%Z) Mk_annot; Val (Val_Bits [BV{64%N} 0xfffffffffffff000%Z]) Mk_annot] Mk_annot; Val (Val_Bits [BV{64%N} 0x0%Z]) Mk_annot] Mk_annot; Val (Val_Bits [BV{64%N} 0x0%Z]) Mk_annot] Mk_annot)) Mk_annot :t:
+  WriteReg "R1" [] (RegVal_Base (Val_Symbolic 40%Z)) Mk_annot :t:
+  Smt (DefineConst 41%Z (Manyop (Bvmanyarith Bvadd) [Val (Val_Symbolic 37%Z) Mk_annot; Val (Val_Bits [BV{64%N} 0x4%Z]) Mk_annot] Mk_annot)) Mk_annot :t:
+  WriteReg "_PC" [] (RegVal_Base (Val_Symbolic 41%Z)) Mk_annot :t:
+  tnil
+.
