instructions/hello/a1c.v
@@ -1,47 +1,42 @@
-From isla Require Import isla_lang.
+From isla Require Import opsem.
 
-Definition a1c : list trc := [
-  [
-    Smt (DeclareConst 36%Z (Ty_BitVec 64%N)) Mk_annot;
-    ReadReg "R0" [] (RegVal_Base (Val_Symbolic 36%Z)) Mk_annot;
-    Smt (DefineConst 39%Z (Binop (Eq) (Binop (Eq) (Unop (Extract 31%N 0%N) (Val (Val_Symbolic 36%Z) Mk_annot) Mk_annot) (Val (Val_Bits [BV{32%N} 0x0%Z]) Mk_annot) Mk_annot) (Val (Val_Bool false) Mk_annot) Mk_annot)) Mk_annot;
-    Branch 0%Z "model/aarch64.sail 12148:4 - 12150:5" Mk_annot;
-    Smt (Assert (Unop (Not) (Val (Val_Symbolic 39%Z) Mk_annot) Mk_annot)) Mk_annot;
-    Smt (DeclareConst 40%Z (Ty_BitVec 64%N)) Mk_annot;
-    ReadReg "_PC" [] (RegVal_Base (Val_Symbolic 40%Z)) Mk_annot;
-    Smt (DefineConst 41%Z (Manyop (Bvmanyarith Bvadd) [Val (Val_Symbolic 40%Z) Mk_annot; Val (Val_Bits [BV{64%N} 0x4%Z]) Mk_annot] Mk_annot)) Mk_annot;
-    WriteReg "_PC" [] (RegVal_Base (Val_Symbolic 41%Z)) Mk_annot
-  ];
-  [
-    AssumeReg "HCR_EL2" [] (RegVal_Base (Val_Bits [BV{64%N} 0x80000000%Z])) Mk_annot;
-    AssumeReg "CFG_ID_AA64PFR0_EL1_EL3" [] (RegVal_Base (Val_Bits [BV{4%N} 0x1%Z])) Mk_annot;
-    AssumeReg "CFG_ID_AA64PFR0_EL1_EL2" [] (RegVal_Base (Val_Bits [BV{4%N} 0x1%Z])) Mk_annot;
-    AssumeReg "CFG_ID_AA64PFR0_EL1_EL1" [] (RegVal_Base (Val_Bits [BV{4%N} 0x1%Z])) Mk_annot;
-    AssumeReg "CFG_ID_AA64PFR0_EL1_EL0" [] (RegVal_Base (Val_Bits [BV{4%N} 0x1%Z])) Mk_annot;
-    AssumeReg "TCR_EL2" [] (RegVal_Base (Val_Bits [BV{64%N} 0x0%Z])) Mk_annot;
-    AssumeReg "PSTATE" [Field "EL"] (RegVal_Base (Val_Bits [BV{2%N} 0x2%Z])) Mk_annot;
-    AssumeReg "PSTATE" [Field "nRW"] (RegVal_Base (Val_Bits [BV{1%N} 0x0%Z])) Mk_annot;
-    AssumeReg "SCR_EL3" [] (RegVal_Base (Val_Bits [BV{32%N} 0x401%Z])) Mk_annot;
-    Smt (DeclareConst 36%Z (Ty_BitVec 64%N)) Mk_annot;
-    ReadReg "R0" [] (RegVal_Base (Val_Symbolic 36%Z)) Mk_annot;
-    Smt (DefineConst 39%Z (Binop (Eq) (Binop (Eq) (Unop (Extract 31%N 0%N) (Val (Val_Symbolic 36%Z) Mk_annot) Mk_annot) (Val (Val_Bits [BV{32%N} 0x0%Z]) Mk_annot) Mk_annot) (Val (Val_Bool false) Mk_annot) Mk_annot)) Mk_annot;
-    Branch 0%Z "model/aarch64.sail 12148:4 - 12150:5" Mk_annot;
-    Smt (Assert (Val (Val_Symbolic 39%Z) Mk_annot)) Mk_annot;
-    Smt (DeclareConst 40%Z (Ty_BitVec 64%N)) Mk_annot;
-    ReadReg "_PC" [] (RegVal_Base (Val_Symbolic 40%Z)) Mk_annot;
-    Smt (DefineConst 41%Z (Manyop (Bvmanyarith Bvadd) [Val (Val_Symbolic 40%Z) Mk_annot; Val (Val_Bits [BV{64%N} 0xfffffffffffffff8%Z]) Mk_annot] Mk_annot)) Mk_annot;
-    ReadReg "PSTATE" [Field "nRW"] (RegVal_Struct [("nRW", RegVal_Base (Val_Bits [BV{1%N} 0x0%Z]))]) Mk_annot;
-    ReadReg "CFG_ID_AA64PFR0_EL1_EL0" [] (RegVal_Base (Val_Bits [BV{4%N} 0x1%Z])) Mk_annot;
-    ReadReg "CFG_ID_AA64PFR0_EL1_EL1" [] (RegVal_Base (Val_Bits [BV{4%N} 0x1%Z])) Mk_annot;
-    ReadReg "CFG_ID_AA64PFR0_EL1_EL2" [] (RegVal_Base (Val_Bits [BV{4%N} 0x1%Z])) Mk_annot;
-    ReadReg "CFG_ID_AA64PFR0_EL1_EL3" [] (RegVal_Base (Val_Bits [BV{4%N} 0x1%Z])) Mk_annot;
-    Smt (DefineConst 53%Z (Val (Val_Symbolic 41%Z) Mk_annot)) Mk_annot;
-    BranchAddress (RegVal_Base (Val_Symbolic 53%Z)) Mk_annot;
-    Smt (DefineConst 54%Z (Val (Val_Symbolic 41%Z) Mk_annot)) Mk_annot;
-    ReadReg "PSTATE" [Field "EL"] (RegVal_Struct [("EL", RegVal_Base (Val_Bits [BV{2%N} 0x2%Z]))]) Mk_annot;
-    ReadReg "SCR_EL3" [] (RegVal_Base (Val_Bits [BV{32%N} 0x401%Z])) Mk_annot;
-    ReadReg "HCR_EL2" [] (RegVal_Base (Val_Bits [BV{64%N} 0x80000000%Z])) Mk_annot;
-    ReadReg "TCR_EL2" [] (RegVal_Base (Val_Bits [BV{64%N} 0x0%Z])) Mk_annot;
-    WriteReg "_PC" [] (RegVal_Base (Val_Symbolic 54%Z)) Mk_annot
+Definition a1c : isla_trace :=
+  AssumeReg "HCR_EL2" [] (RegVal_Base (Val_Bits [BV{64%N} 0x80000000%Z])) Mk_annot :t:
+  AssumeReg "CFG_ID_AA64PFR0_EL1_EL3" [] (RegVal_Base (Val_Bits [BV{4%N} 0x1%Z])) Mk_annot :t:
+  AssumeReg "CFG_ID_AA64PFR0_EL1_EL2" [] (RegVal_Base (Val_Bits [BV{4%N} 0x1%Z])) Mk_annot :t:
+  AssumeReg "CFG_ID_AA64PFR0_EL1_EL1" [] (RegVal_Base (Val_Bits [BV{4%N} 0x1%Z])) Mk_annot :t:
+  AssumeReg "CFG_ID_AA64PFR0_EL1_EL0" [] (RegVal_Base (Val_Bits [BV{4%N} 0x1%Z])) Mk_annot :t:
+  AssumeReg "TCR_EL2" [] (RegVal_Base (Val_Bits [BV{64%N} 0x0%Z])) Mk_annot :t:
+  AssumeReg "PSTATE" [Field "EL"] (RegVal_Base (Val_Bits [BV{2%N} 0x2%Z])) Mk_annot :t:
+  AssumeReg "PSTATE" [Field "nRW"] (RegVal_Base (Val_Bits [BV{1%N} 0x0%Z])) Mk_annot :t:
+  AssumeReg "SCR_EL3" [] (RegVal_Base (Val_Bits [BV{32%N} 0x401%Z])) Mk_annot :t:
+  Smt (DeclareConst 36%Z (Ty_BitVec 64%N)) Mk_annot :t:
+  ReadReg "R0" [] (RegVal_Base (Val_Symbolic 36%Z)) Mk_annot :t:
+  Smt (DefineConst 39%Z (Binop (Eq) (Binop (Eq) (Unop (Extract 31%N 0%N) (Val (Val_Symbolic 36%Z) Mk_annot) Mk_annot) (Val (Val_Bits [BV{32%N} 0x0%Z]) Mk_annot) Mk_annot) (Val (Val_Bool false) Mk_annot) Mk_annot)) Mk_annot :t:
+  tfork [
+    Smt (Assert (Val (Val_Symbolic 39%Z) Mk_annot)) Mk_annot :t:
+    Smt (DeclareConst 40%Z (Ty_BitVec 64%N)) Mk_annot :t:
+    ReadReg "_PC" [] (RegVal_Base (Val_Symbolic 40%Z)) Mk_annot :t:
+    Smt (DefineConst 41%Z (Manyop (Bvmanyarith Bvadd) [Val (Val_Symbolic 40%Z) Mk_annot; Val (Val_Bits [BV{64%N} 0xfffffffffffffff8%Z]) Mk_annot] Mk_annot)) Mk_annot :t:
+    ReadReg "PSTATE" [Field "nRW"] (RegVal_Struct [("nRW", RegVal_Base (Val_Bits [BV{1%N} 0x0%Z]))]) Mk_annot :t:
+    ReadReg "CFG_ID_AA64PFR0_EL1_EL0" [] (RegVal_Base (Val_Bits [BV{4%N} 0x1%Z])) Mk_annot :t:
+    ReadReg "CFG_ID_AA64PFR0_EL1_EL1" [] (RegVal_Base (Val_Bits [BV{4%N} 0x1%Z])) Mk_annot :t:
+    ReadReg "CFG_ID_AA64PFR0_EL1_EL2" [] (RegVal_Base (Val_Bits [BV{4%N} 0x1%Z])) Mk_annot :t:
+    ReadReg "CFG_ID_AA64PFR0_EL1_EL3" [] (RegVal_Base (Val_Bits [BV{4%N} 0x1%Z])) Mk_annot :t:
+    Smt (DefineConst 53%Z (Val (Val_Symbolic 41%Z) Mk_annot)) Mk_annot :t:
+    BranchAddress (RegVal_Base (Val_Symbolic 53%Z)) Mk_annot :t:
+    Smt (DefineConst 54%Z (Val (Val_Symbolic 41%Z) Mk_annot)) Mk_annot :t:
+    ReadReg "PSTATE" [Field "EL"] (RegVal_Struct [("EL", RegVal_Base (Val_Bits [BV{2%N} 0x2%Z]))]) Mk_annot :t:
+    ReadReg "SCR_EL3" [] (RegVal_Base (Val_Bits [BV{32%N} 0x401%Z])) Mk_annot :t:
+    ReadReg "HCR_EL2" [] (RegVal_Base (Val_Bits [BV{64%N} 0x80000000%Z])) Mk_annot :t:
+    ReadReg "TCR_EL2" [] (RegVal_Base (Val_Bits [BV{64%N} 0x0%Z])) Mk_annot :t:
+    WriteReg "_PC" [] (RegVal_Base (Val_Symbolic 54%Z)) Mk_annot :t:
+    tnil;
+    Smt (Assert (Unop (Not) (Val (Val_Symbolic 39%Z) Mk_annot) Mk_annot)) Mk_annot :t:
+    Smt (DeclareConst 40%Z (Ty_BitVec 64%N)) Mk_annot :t:
+    ReadReg "_PC" [] (RegVal_Base (Val_Symbolic 40%Z)) Mk_annot :t:
+    Smt (DefineConst 41%Z (Manyop (Bvmanyarith Bvadd) [Val (Val_Symbolic 40%Z) Mk_annot; Val (Val_Bits [BV{64%N} 0x4%Z]) Mk_annot] Mk_annot)) Mk_annot :t:
+    WriteReg "_PC" [] (RegVal_Base (Val_Symbolic 41%Z)) Mk_annot :t:
+    tnil
   ]
-].
+.
