instructions/uart/a8016c.v
@@ -1,14 +1,13 @@
-From isla Require Import isla_lang.
+From isla Require Import opsem.
 
-Definition a8016c : list trc := [
-  [
-    Smt (DeclareConst 53%Z (Ty_BitVec 64%N)) Mk_annot;
-    ReadReg "R0" [] (RegVal_Base (Val_Symbolic 53%Z)) Mk_annot;
-    Smt (DefineConst 56%Z (Manyop Concat [Val (Val_Bits [BV{32%N} 0x0%Z]) Mk_annot; Manyop (Bvmanyarith Bvand) [Unop (Extract 31%N 0%N) (Val (Val_Symbolic 53%Z) Mk_annot) Mk_annot; Val (Val_Bits [BV{32%N} 0xff%Z]) Mk_annot] Mk_annot] Mk_annot)) Mk_annot;
-    WriteReg "R0" [] (RegVal_Base (Val_Symbolic 56%Z)) Mk_annot;
-    Smt (DeclareConst 57%Z (Ty_BitVec 64%N)) Mk_annot;
-    ReadReg "_PC" [] (RegVal_Base (Val_Symbolic 57%Z)) Mk_annot;
-    Smt (DefineConst 58%Z (Manyop (Bvmanyarith Bvadd) [Val (Val_Symbolic 57%Z) Mk_annot; Val (Val_Bits [BV{64%N} 0x4%Z]) Mk_annot] Mk_annot)) Mk_annot;
-    WriteReg "_PC" [] (RegVal_Base (Val_Symbolic 58%Z)) Mk_annot
-  ]
-].
+Definition a8016c : isla_trace :=
+  Smt (DeclareConst 53%Z (Ty_BitVec 64%N)) Mk_annot :t:
+  ReadReg "R0" [] (RegVal_Base (Val_Symbolic 53%Z)) Mk_annot :t:
+  Smt (DefineConst 56%Z (Manyop Concat [Val (Val_Bits [BV{32%N} 0x0%Z]) Mk_annot; Manyop (Bvmanyarith Bvand) [Unop (Extract 31%N 0%N) (Val (Val_Symbolic 53%Z) Mk_annot) Mk_annot; Val (Val_Bits [BV{32%N} 0xff%Z]) Mk_annot] Mk_annot] Mk_annot)) Mk_annot :t:
+  WriteReg "R0" [] (RegVal_Base (Val_Symbolic 56%Z)) Mk_annot :t:
+  Smt (DeclareConst 57%Z (Ty_BitVec 64%N)) Mk_annot :t:
+  ReadReg "_PC" [] (RegVal_Base (Val_Symbolic 57%Z)) Mk_annot :t:
+  Smt (DefineConst 58%Z (Manyop (Bvmanyarith Bvadd) [Val (Val_Symbolic 57%Z) Mk_annot; Val (Val_Bits [BV{64%N} 0x4%Z]) Mk_annot] Mk_annot)) Mk_annot :t:
+  WriteReg "_PC" [] (RegVal_Base (Val_Symbolic 58%Z)) Mk_annot :t:
+  tnil
+.
