pkvm_handler/a7408.v
@@ -1,15 +1,14 @@
-From isla Require Import isla_lang.
+From isla Require Import opsem.
 
-Definition a7408 : list trc := [
-  [
-    Smt (DeclareConst 49%Z (Ty_BitVec 64%N)) Mk_annot;
-    ReadReg "R0" [] (RegVal_Base (Val_Symbolic 49%Z)) Mk_annot;
-    Smt (DefineConst 50%Z (Val (Val_Symbolic 49%Z) Mk_annot)) Mk_annot;
-    Smt (DefineConst 73%Z (Manyop (Bvmanyarith Bvor) [Val (Val_Bits [BV{64%N} 0x0%Z]) Mk_annot; Manyop (Bvmanyarith Bvand) [Manyop (Bvmanyarith Bvor) [Val (Val_Bits [BV{64%N} 0x0%Z]) Mk_annot; Manyop (Bvmanyarith Bvand) [Manyop (Bvmanyarith Bvor) [Binop ((Bvarith Bvlshr)) (Val (Val_Symbolic 50%Z) Mk_annot) (Val (Val_Bits [BV{64%N} 0x1a%Z]) Mk_annot) Mk_annot; Binop ((Bvarith Bvshl)) (Val (Val_Symbolic 50%Z) Mk_annot) (Val (Val_Bits [BV{64%N} 0x26%Z]) Mk_annot) Mk_annot] Mk_annot; Val (Val_Bits [BV{64%N} 0xffffffffffffffff%Z]) Mk_annot] Mk_annot] Mk_annot; Val (Val_Bits [BV{64%N} 0x3fffffffff%Z]) Mk_annot] Mk_annot] Mk_annot)) Mk_annot;
-    WriteReg "R0" [] (RegVal_Base (Val_Symbolic 73%Z)) Mk_annot;
-    Smt (DeclareConst 74%Z (Ty_BitVec 64%N)) Mk_annot;
-    ReadReg "_PC" [] (RegVal_Base (Val_Symbolic 74%Z)) Mk_annot;
-    Smt (DefineConst 75%Z (Manyop (Bvmanyarith Bvadd) [Val (Val_Symbolic 74%Z) Mk_annot; Val (Val_Bits [BV{64%N} 0x4%Z]) Mk_annot] Mk_annot)) Mk_annot;
-    WriteReg "_PC" [] (RegVal_Base (Val_Symbolic 75%Z)) Mk_annot
-  ]
-].
+Definition a7408 : isla_trace :=
+  Smt (DeclareConst 49%Z (Ty_BitVec 64%N)) Mk_annot :t:
+  ReadReg "R0" [] (RegVal_Base (Val_Symbolic 49%Z)) Mk_annot :t:
+  Smt (DefineConst 50%Z (Val (Val_Symbolic 49%Z) Mk_annot)) Mk_annot :t:
+  Smt (DefineConst 73%Z (Manyop (Bvmanyarith Bvor) [Val (Val_Bits [BV{64%N} 0x0%Z]) Mk_annot; Manyop (Bvmanyarith Bvand) [Manyop (Bvmanyarith Bvor) [Val (Val_Bits [BV{64%N} 0x0%Z]) Mk_annot; Manyop (Bvmanyarith Bvand) [Manyop (Bvmanyarith Bvor) [Binop ((Bvarith Bvlshr)) (Val (Val_Symbolic 50%Z) Mk_annot) (Val (Val_Bits [BV{64%N} 0x1a%Z]) Mk_annot) Mk_annot; Binop ((Bvarith Bvshl)) (Val (Val_Symbolic 50%Z) Mk_annot) (Val (Val_Bits [BV{64%N} 0x26%Z]) Mk_annot) Mk_annot] Mk_annot; Val (Val_Bits [BV{64%N} 0xffffffffffffffff%Z]) Mk_annot] Mk_annot] Mk_annot; Val (Val_Bits [BV{64%N} 0x3fffffffff%Z]) Mk_annot] Mk_annot] Mk_annot)) Mk_annot :t:
+  WriteReg "R0" [] (RegVal_Base (Val_Symbolic 73%Z)) Mk_annot :t:
+  Smt (DeclareConst 74%Z (Ty_BitVec 64%N)) Mk_annot :t:
+  ReadReg "_PC" [] (RegVal_Base (Val_Symbolic 74%Z)) Mk_annot :t:
+  Smt (DefineConst 75%Z (Manyop (Bvmanyarith Bvadd) [Val (Val_Symbolic 74%Z) Mk_annot; Val (Val_Bits [BV{64%N} 0x4%Z]) Mk_annot] Mk_annot)) Mk_annot :t:
+  WriteReg "_PC" [] (RegVal_Base (Val_Symbolic 75%Z)) Mk_annot :t:
+  tnil
+.
