pkvm_handler/a7420.v
@@ -1,18 +1,17 @@
-From isla Require Import isla_lang.
+From isla Require Import opsem.
 
-Definition a7420 : list trc := [
-  [
-    AssumeReg "PSTATE" [Field "EL"] (RegVal_Base (Val_Bits [BV{2%N} 0x2%Z])) Mk_annot;
-    AssumeReg "PSTATE" [Field "SP"] (RegVal_Base (Val_Bits [BV{1%N} 0x1%Z])) Mk_annot;
-    ReadReg "PSTATE" [Field "SP"] (RegVal_Struct [("SP", RegVal_Base (Val_Bits [BV{1%N} 0x1%Z]))]) Mk_annot;
-    ReadReg "PSTATE" [Field "EL"] (RegVal_Struct [("EL", RegVal_Base (Val_Bits [BV{2%N} 0x2%Z]))]) Mk_annot;
-    Smt (DeclareConst 38%Z (Ty_BitVec 64%N)) Mk_annot;
-    ReadReg "SP_EL2" [] (RegVal_Base (Val_Symbolic 38%Z)) Mk_annot;
-    Smt (DefineConst 61%Z (Manyop (Bvmanyarith Bvadd) [Unop (Extract 63%N 0%N) (Unop (ZeroExtend 64%N) (Val (Val_Symbolic 38%Z) Mk_annot) Mk_annot) Mk_annot; Val (Val_Bits [BV{64%N} 0x10%Z]) Mk_annot] Mk_annot)) Mk_annot;
-    WriteReg "SP_EL2" [] (RegVal_Base (Val_Symbolic 61%Z)) Mk_annot;
-    Smt (DeclareConst 62%Z (Ty_BitVec 64%N)) Mk_annot;
-    ReadReg "_PC" [] (RegVal_Base (Val_Symbolic 62%Z)) Mk_annot;
-    Smt (DefineConst 63%Z (Manyop (Bvmanyarith Bvadd) [Val (Val_Symbolic 62%Z) Mk_annot; Val (Val_Bits [BV{64%N} 0x4%Z]) Mk_annot] Mk_annot)) Mk_annot;
-    WriteReg "_PC" [] (RegVal_Base (Val_Symbolic 63%Z)) Mk_annot
-  ]
-].
+Definition a7420 : isla_trace :=
+  AssumeReg "PSTATE" [Field "EL"] (RegVal_Base (Val_Bits [BV{2%N} 0x2%Z])) Mk_annot :t:
+  AssumeReg "PSTATE" [Field "SP"] (RegVal_Base (Val_Bits [BV{1%N} 0x1%Z])) Mk_annot :t:
+  ReadReg "PSTATE" [Field "SP"] (RegVal_Struct [("SP", RegVal_Base (Val_Bits [BV{1%N} 0x1%Z]))]) Mk_annot :t:
+  ReadReg "PSTATE" [Field "EL"] (RegVal_Struct [("EL", RegVal_Base (Val_Bits [BV{2%N} 0x2%Z]))]) Mk_annot :t:
+  Smt (DeclareConst 38%Z (Ty_BitVec 64%N)) Mk_annot :t:
+  ReadReg "SP_EL2" [] (RegVal_Base (Val_Symbolic 38%Z)) Mk_annot :t:
+  Smt (DefineConst 61%Z (Manyop (Bvmanyarith Bvadd) [Unop (Extract 63%N 0%N) (Unop (ZeroExtend 64%N) (Val (Val_Symbolic 38%Z) Mk_annot) Mk_annot) Mk_annot; Val (Val_Bits [BV{64%N} 0x10%Z]) Mk_annot] Mk_annot)) Mk_annot :t:
+  WriteReg "SP_EL2" [] (RegVal_Base (Val_Symbolic 61%Z)) Mk_annot :t:
+  Smt (DeclareConst 62%Z (Ty_BitVec 64%N)) Mk_annot :t:
+  ReadReg "_PC" [] (RegVal_Base (Val_Symbolic 62%Z)) Mk_annot :t:
+  Smt (DefineConst 63%Z (Manyop (Bvmanyarith Bvadd) [Val (Val_Symbolic 62%Z) Mk_annot; Val (Val_Bits [BV{64%N} 0x4%Z]) Mk_annot] Mk_annot)) Mk_annot :t:
+  WriteReg "_PC" [] (RegVal_Base (Val_Symbolic 63%Z)) Mk_annot :t:
+  tnil
+.
