pkvm_handler/a7430.v
@@ -1,14 +1,13 @@
-From isla Require Import isla_lang.
+From isla Require Import opsem.
 
-Definition a7430 : list trc := [
-  [
-    Smt (DeclareConst 44%Z (Ty_BitVec 64%N)) Mk_annot;
-    ReadReg "R6" [] (RegVal_Base (Val_Symbolic 44%Z)) Mk_annot;
-    Smt (DefineConst 47%Z (Manyop (Bvmanyarith Bvor) [Manyop (Bvmanyarith Bvand) [Val (Val_Symbolic 44%Z) Mk_annot; Val (Val_Bits [BV{64%N} 0xffff0000ffffffff%Z]) Mk_annot] Mk_annot; Val (Val_Bits [BV{64%N} 0x0%Z]) Mk_annot] Mk_annot)) Mk_annot;
-    WriteReg "R6" [] (RegVal_Base (Val_Symbolic 47%Z)) Mk_annot;
-    Smt (DeclareConst 48%Z (Ty_BitVec 64%N)) Mk_annot;
-    ReadReg "_PC" [] (RegVal_Base (Val_Symbolic 48%Z)) Mk_annot;
-    Smt (DefineConst 49%Z (Manyop (Bvmanyarith Bvadd) [Val (Val_Symbolic 48%Z) Mk_annot; Val (Val_Bits [BV{64%N} 0x4%Z]) Mk_annot] Mk_annot)) Mk_annot;
-    WriteReg "_PC" [] (RegVal_Base (Val_Symbolic 49%Z)) Mk_annot
-  ]
-].
+Definition a7430 : isla_trace :=
+  Smt (DeclareConst 44%Z (Ty_BitVec 64%N)) Mk_annot :t:
+  ReadReg "R6" [] (RegVal_Base (Val_Symbolic 44%Z)) Mk_annot :t:
+  Smt (DefineConst 47%Z (Manyop (Bvmanyarith Bvor) [Manyop (Bvmanyarith Bvand) [Val (Val_Symbolic 44%Z) Mk_annot; Val (Val_Bits [BV{64%N} 0xffff0000ffffffff%Z]) Mk_annot] Mk_annot; Val (Val_Bits [BV{64%N} 0x0%Z]) Mk_annot] Mk_annot)) Mk_annot :t:
+  WriteReg "R6" [] (RegVal_Base (Val_Symbolic 47%Z)) Mk_annot :t:
+  Smt (DeclareConst 48%Z (Ty_BitVec 64%N)) Mk_annot :t:
+  ReadReg "_PC" [] (RegVal_Base (Val_Symbolic 48%Z)) Mk_annot :t:
+  Smt (DefineConst 49%Z (Manyop (Bvmanyarith Bvadd) [Val (Val_Symbolic 48%Z) Mk_annot; Val (Val_Bits [BV{64%N} 0x4%Z]) Mk_annot] Mk_annot)) Mk_annot :t:
+  WriteReg "_PC" [] (RegVal_Base (Val_Symbolic 49%Z)) Mk_annot :t:
+  tnil
+.
